theories/InstantiateI.v
@@ -1,0 +1,48 @@
+Require Import Coq.Lists.List.
+Require Import ExtLib.Data.HList.
+Require Import MirrorCore.EnvI.
+Require Import MirrorCore.ExprI.
+Require Import MirrorCore.TypesI.
+
+Section definitions.
+  Variables typ expr : Type.
+  Context {RType_typ : RType typ}.
+  Context {Expr_expr : Expr _ expr}.
+  Context {ExprOk_expr : ExprOk Expr_expr}.
+
+  (** instantiate **)
+  Variable instantiate : (nat -> option expr) -> nat -> expr -> expr.
+
+  Definition sem_preserves_if tus tvs
+             (P : hlist _ tus -> hlist _ tvs -> Prop)
+             (f : nat -> option expr) : Prop :=
+    forall u e t get,
+      f u = Some e ->
+      nth_error_get_hlist_nth _ tus u = Some (@existT _ _ t get) ->
+      exists eD,
+        exprD' tus tvs e t = Some eD /\
+        forall us vs,
+          P us vs ->
+          get us = eD us vs.
+
+  Definition instantiate_mentionsU : Prop :=
+    forall f n e u,
+      mentionsU u (instantiate f n e) = true <-> (** do i need iff? **)
+      (   (f u = None /\ mentionsU u e = true)
+       \/ exists u' e',
+            f u' = Some e' /\
+            mentionsU u' e = true/\
+            mentionsU u e' = true).
+
+  Definition exprD'_instantiate : Prop :=
+    forall tus tvs f e tvs' t eD P,
+      sem_preserves_if tus tvs P f ->
+      exprD' tus (tvs' ++ tvs) e t = Some eD ->
+      exists eD',
+        exprD' tus (tvs' ++ tvs) (instantiate f (length tvs') e) t = Some eD' /\
+        forall us vs vs',
+          P us vs ->
+          eD us (hlist_app vs' vs) = eD' us (hlist_app vs' vs).
+End definitions.
+
+Arguments sem_preserves_if {typ expr RType Expr} _ _ _ _ : rename.
