theories/Lambda/ExprUnify_simul.v
@@ -2,6 +2,7 @@ Require Import Coq.Lists.List.
 Require Import ExtLib.Core.RelDec.
 Require Import ExtLib.Data.ListNth.
 Require Import ExtLib.Data.HList.
+Require Import ExtLib.Data.Option.
 Require Import ExtLib.Data.Fun.
 Require Import ExtLib.Data.Eq.
 Require Import ExtLib.Data.Pair.
