theories/Util/ListMapT.v
@@ -1,0 +1,111 @@
+Require Import ExtLib.Structures.Traversable.
+Require Import ExtLib.Structures.Applicative.
+Require Import ExtLib.Data.List.
+Require Import ExtLib.Data.Option.
+Require Import ExtLib.Tactics.
+
+Set Implicit Arguments.
+Set Strict Implict.
+
+Section mapT_equations.
+  Variables T U : Type.
+
+  Lemma list_mapT_cons
+  : forall (F : T -> option U) ls a,
+      Traversable.mapT F (a :: ls) =
+      match match F a with
+              | Some x => Some (cons x)
+              | None => None
+            end with
+        | Some f =>
+          match Traversable.mapT F ls with
+            | Some x => Some (f x)
+            | None => None
+          end
+        | None => None
+      end.
+  Proof. reflexivity. Qed.
+
+  Lemma list_mapT_nil
+  : forall (F : T -> option U),
+      Traversable.mapT F nil = Some nil.
+  Proof. reflexivity. Qed.
+End mapT_equations.
+
+Section mapT_facts.
+  Variables T U : Type.
+
+  Lemma mapT_In
+  : forall (f : T -> option U) ls ls' x,
+      mapT f ls = Some ls' ->
+      In x ls' ->
+      exists y, f y = Some x /\ In y ls.
+  Proof.
+    clear.
+    induction ls.
+    { simpl. intros; inv_all; subst. destruct H0. }
+    { intros. rewrite list_mapT_cons in H.
+      forward. inv_all. subst.
+      destruct H0.
+      { subst. eexists; split; eauto. left. reflexivity. }
+      { eapply IHls in H0; eauto.
+        forward_reason. eexists; split; eauto. right; assumption. } }
+  Qed.
+
+  Lemma mapT_map
+  : forall V (f : U -> option V) (g : T -> U) ls,
+      mapT f (map g ls) = mapT (fun x => f (g x)) ls.
+  Proof.
+    clear. induction ls; try solve [ simpl; auto ].
+    simpl map. do 2 rewrite list_mapT_cons.
+    destruct (f (g a)); auto.
+    rewrite IHls. reflexivity.
+  Qed.
+
+  Lemma map_mapT
+  : forall V (f : T -> option U) (g : U -> V) ls,
+      match mapT f ls with
+        | None => None
+        | Some x => Some (map g x)
+      end = mapT (fun x => match f x with
+                             | None => None
+                             | Some x => Some (g x)
+                           end) ls.
+  Proof.
+    clear. induction ls; auto.
+    do 2 rewrite list_mapT_cons.
+    destruct (f a); auto.
+    rewrite <- IHls.
+    destruct (mapT f ls); auto.
+  Qed.
+
+  Lemma mapT_ext
+  : forall T U (f g : T -> option U),
+      (forall x, f x = g x) ->
+      forall (ls : list T),
+        mapT f ls = mapT g ls.
+  Proof.
+    clear. induction ls; auto; intros.
+    do 2 rewrite list_mapT_cons.
+    rewrite H. rewrite IHls. destruct (g a); auto.
+  Qed.
+
+  Lemma mapT_success
+  : forall (f : T -> option U) ls ls',
+      mapT f ls = Some ls' ->
+      forall x, In x ls ->
+                exists y, f x = Some y /\ In y ls'.
+  Proof.
+    clear. induction ls.
+    { rewrite list_mapT_nil. intros.
+      inv_all; subst. destruct H0. }
+    { rewrite list_mapT_cons.
+      intros. forward. inv_all; subst.
+      destruct H0.
+      { subst. eexists; split; eauto. left. reflexivity. }
+      { eapply IHls in H0; [ | reflexivity ].
+        forward_reason. eexists; split; eauto.
+        right. assumption. } }
+  Qed.
+
+End mapT_facts.
